rocq/ZF/Meta/DeclP.v
@@ -7,15 +7,11 @@ Require Import ZF.Meta.Ty.
 Import ListNotations.
 
 (* A proof declaration records parameters, conclusion and proof body.           *)
-Record Decl : Type := mkDecl
+Record DeclP : Type := mkDeclP
   { paraP  : list Ty
   ; conclP : Term
   ; bodyP  : Proof
   }.
 
 (* A proof declaration conclusion is checked in de Bruijn context order.        *)
-Definition ctx (d:Decl) : Ctx := rev (paraP d).
-
-Definition DeclP    := Decl.
-Definition mkDeclP  := mkDecl.
-Definition ctxP     := ctx.
+Definition ctxP (d:DeclP) : Ctx := rev (paraP d).
