rocq/ZF/Meta/DeclT.v
@@ -7,15 +7,11 @@ Require Import ZF.Meta.Ty.
 Import ListNotations.
 
 (* A term declaration records parameters, result sort and body.                 *)
-Record Decl : Type := mkDecl
+Record DeclT : Type := mkDeclT
   { paraT : list Ty
   ; resT  : Ty
   ; bodyT : Term
   }.
 
 (* A term declaration body is checked in de Bruijn context order.               *)
-Definition ctx (d:Decl) : Ctx := rev (paraT d).
-
-Definition DeclT      := Decl.
-Definition mkDeclT    := mkDecl.
-Definition ctxT       := ctx.
+Definition ctxT (d:DeclT) : Ctx := rev (paraT d).
