rocq/ZF/Meta/CheckDeclP.v
@@ -1,0 +1,9 @@
+Require Import ZF.Meta.Check.
+Require Import ZF.Meta.DeclP.
+Require Import ZF.Meta.Env.
+Require Import ZF.Meta.Ty.
+
+(* A proof declaration is checked when its conclusion has a proof.              *)
+Definition CheckP (E:Env) (d:DeclP) : Prop :=
+  CheckT E (ctxP d) (conclP d) TyProp /\
+  CheckP E (ctxP d) (bodyP d) (conclP d).
