rocq/ZF/Meta/CheckDeclT.v
@@ -1,0 +1,7 @@
+Require Import ZF.Meta.Check.
+Require Import ZF.Meta.DeclT.
+Require Import ZF.Meta.Env.
+
+(* A term declaration is checked when its body has its declared sort.           *)
+Definition CheckT (E:Env) (d:DeclT) : Prop :=
+  CheckT E (ctxT d) (bodyT d) (resT d).
