rocq/ZF/Meta/Decl/Class/Cardinal/Aleph.v
@@ -3,7 +3,7 @@ Require Import Coq.Strings.String.
 
 Require Import ZF.Meta.Env.
 Require Import ZF.Meta.Syntax.
-Require Import ZF.Meta.Term.Decl.
+Require Import ZF.Meta.DeclT.
 Require Import ZF.Meta.Ty.
 
 Import ListNotations.
