rocq/ZF/Meta/Decl/Class/Incl.v
@@ -2,9 +2,9 @@ Require Import Coq.Lists.List.
 Require Import Coq.Strings.String.
 
 Require Import ZF.Meta.Env.
-Require Import ZF.Meta.Proof.Decl.
+Require Import ZF.Meta.DeclP.
 Require Import ZF.Meta.Syntax.
-Require Import ZF.Meta.Term.Decl.
+Require Import ZF.Meta.DeclT.
 Require Import ZF.Meta.Ty.
 
 Import ListNotations.
