rocq/ZF/Meta/Decl/Set/Relation/FunctionOn.v
@@ -4,7 +4,7 @@ Require Import Coq.Strings.String.
 Require Import ZF.Meta.Env.
 Require Import ZF.Meta.Env.
 Require Import ZF.Meta.Syntax.
-Require Import ZF.Meta.Term.Decl.
+Require Import ZF.Meta.DeclT.
 Require Import ZF.Meta.Ty.
 
 Import ListNotations.
