rocq/ZF/Meta/Test/Axiom/NonEmptyUniverse.v
@@ -3,8 +3,8 @@ Require Import Coq.Strings.String.
 
 Require Import ZF.Meta.Syntax.
 Require Import ZF.Meta.Check.
-Require Import ZF.Meta.Proof.CheckDecl.
-Require Import ZF.Meta.Proof.Decl.
+Require Import ZF.Meta.CheckDeclP.
+Require Import ZF.Meta.DeclP.
 Require Import ZF.Meta.Ty.
 
 Import ListNotations.
@@ -13,10 +13,10 @@ Open Scope string_scope.
 Require Import ZF.Meta.Decl.Axiom.NonEmptyUniverse.
 
 Proposition NonEmptyUniverse :
-  CheckDeclP (NonEmptyUniverse.env) NonEmptyUniverse.
+  CheckP (NonEmptyUniverse.env) NonEmptyUniverse.
 Proof.
   (* Proof by Hermes + gpt 5.5                                                  *)
-  assert (CheckT NonEmptyUniverse.env []
+  assert (Check.CheckT NonEmptyUniverse.env []
     (conclP NonEmptyUniverse) TyProp) as H1. { apply CheckEx, CheckTop. }
   split. 1: assumption. apply CheckAxiomP. assumption.
 Qed.
